AutoKchp/MorphismDfs.lean
@@ -10,115 +10,113 @@ public import AutoKchp.CDFA
 import AutoKchp.Internal.Util
 
 /-
-DFS to find a "state morphism" (which does not necessarily map terminal states to terminal states)
+DFS to find a "state morphism" (which does not necessarily map final states to final states)
 -/
-abbrev DFSTable {a: Nat} (r s: NatCDFA a) := Vector (Option (Fin s.n × List (Fin a))) r.n
+abbrev DFSMap {a: Nat} (r s: CDFA a) := Std.HashMap r.σ (s.σ × List (Fin a))
 
 
 abbrev DFSError (a: Nat) := List (Fin a) × List (Fin a)
 
 
-abbrev DFSResult {a: Nat} (r s: NatCDFA a) := Except (DFSError a) (DFSTable r s)
-
-
-def dfsFindMorphismFrom {a: Nat} (r s: NatCDFA a) (p: Fin r.n) (q: Fin s.n)
-  (l: List (Fin a)) (asgn: DFSTable r s):
-    Nat → DFSResult r s
+def dfsFindMorphismFrom {a: Nat} (r s: CDFA a) (p: r.σ) (q: s.σ)
+  (l: List (Fin a)) (asgn: DFSMap r s):
+    Nat → Except (DFSError a) (DFSMap r s)
   | 0 => Except.error ([], []) --Should be unreachable with enough fuel
   | fuel + 1 =>
-    match asgn.get p with
+    match asgn[p]? with
     | none => Fin.foldlM a
       (fun acc b => dfsFindMorphismFrom r s (r.δ p b) (s.δ q b) (b::l) acc fuel)
-      (asgn.set p (some (q, l)))
+      (asgn.insert p (q, l))
     | some (q', l') => if q' = q then Except.ok asgn else Except.error (l.reverse, l'.reverse)
 
 
-theorem dfsFindMorphismFrom_preserves_some {a: Nat} {r s: NatCDFA a} {p: Fin r.n} {q: Fin s.n}
-  {l: List (Fin a)} {asgn: DFSTable r s} {i: Fin r.n} {v: Fin s.n × List (Fin a)} (h: asgn.get i = some v):
-    {fuel: Nat} → (dfsFindMorphismFrom r s p q l asgn fuel).allP (fun w => w.get i = some v)
+theorem dfsFindMorphismFrom_preserves {a: Nat} {r s: CDFA a} {p: r.σ} {q: s.σ}
+  {l: List (Fin a)} {asgn: DFSMap r s} {i: r.σ} {v: s.σ × List (Fin a)} (h: asgn.get? i = some v):
+    {fuel: Nat} → (dfsFindMorphismFrom r s p q l asgn fuel).allP (fun w => w[i]? = some v)
   | 0 => True.intro
-  | fuel + 1 =>
-    match eq: asgn.get p with
+  | _ + 1 =>
+    match eq: asgn[p]? with
     | none => dfsFindMorphismFrom.eq_def r s p q l asgn _ ▸ eq ▸
         Fin.foldlM_induction (fun (w: Except _ _) _ => w.allP _)
           (have ne: p ≠ i := fun eq2 => Option.some_ne_none v (h.symm.trans (eq2 ▸ eq))
-            have concl: (asgn.set p (some (q, l))).get i = some v :=
-              (Vector.get_set_of_ne ne).trans h
+            have concl: (asgn.insert p (q, l)).get? i = some v :=
+              (Std.HashMap.getElem?_insert_of_ne ne).trans h
             Except.pure_def ▸ concl)
-          (fun acc b hrec =>
+          (fun acc _ hrec =>
             match acc with
             | Except.error _ => True.intro
-            | Except.ok acc => dfsFindMorphismFrom_preserves_some hrec)
-    | some q' => dfsFindMorphismFrom.eq_def r s p q l asgn _ ▸ eq ▸
+            | Except.ok _ => dfsFindMorphismFrom_preserves hrec)
+    | some _ => dfsFindMorphismFrom.eq_def r s p q l asgn _ ▸ eq ▸
         iteInduction (motive := fun w: Except _ _ => w.allP _)
           (fun _ => h) (fun _ => True.intro)
 
 
-theorem dfsFindMorphismFrom_step {a: Nat} {r s: NatCDFA a} {p: Fin r.n} {q: Fin s.n}
-  {l: List (Fin a)} {asgn: DFSTable r s}:
-    {fuel: Nat} → (dfsFindMorphismFrom r s p q l asgn fuel).allP (fun w => ∃ u: List (Fin a), w.get p = some (q, u))
+theorem dfsFindMorphismFrom_step {a: Nat} {r s: CDFA a} {p: r.σ} {q: s.σ}
+  {l: List (Fin a)} {asgn: DFSMap r s}:
+    {fuel: Nat} → (dfsFindMorphismFrom r s p q l asgn fuel).allP
+      (fun w => ∃ u: List (Fin a), w[p]? = some (q, u))
   | 0 => True.intro
   | _ + 1 =>
-    match eq: asgn.get p with
+    match eq: asgn[p]? with
     | none => dfsFindMorphismFrom.eq_def r s p q l asgn _ ▸ eq ▸
         Fin.foldlM_induction (fun (w: Except _ _) _ => w.allP _)
-          (Except.pure_def ▸ ⟨l, Vector.get_set_self⟩)
+          (Except.pure_def ▸ ⟨l, Std.HashMap.getElem?_insert_self⟩)
           (fun acc _ hrec =>
             match acc with
             | Except.error _ => True.intro
             | Except.ok _ =>
               have ⟨u, hu⟩ := hrec
-              Except.allP_mp (dfsFindMorphismFrom_preserves_some hu) (fun _ hu2 => ⟨u, hu2⟩)
+              Except.allP_mp (dfsFindMorphismFrom_preserves hu) (fun _ hu2 => ⟨u, hu2⟩)
           )
     | some (_, l') => dfsFindMorphismFrom.eq_def r s p q l asgn _ ▸ eq ▸
         iteInduction (motive := fun w: Except _ _ => w.allP _)
           (fun eq2 => ⟨l', eq2 ▸ eq⟩) (fun _ => True.intro)
 
 
-def okInvariant {a: Nat} (r s: NatCDFA a)
-  (grey: List (Fin r.n)) (acc: DFSTable r s): Prop :=
-    ∀ p: Fin r.n, p ∉ grey → (acc.get p).allP (fun (q, _) => ∀ b: Fin a, ∃ u: List (Fin a),
-      acc.get (r.δ p b) = some (s.δ q b, u)
+def okInvariant {a: Nat} (r s: CDFA a)
+  (grey: List r.σ) (acc: DFSMap r s): Prop :=
+    ∀ p: r.σ, p ∉ grey → acc[p]?.allP (fun (q, _) => ∀ b: Fin a, ∃ u: List (Fin a),
+      acc[r.δ p b]? = some (s.δ q b, u)
     )
 
 
 --Big ugly theorem (the annoying part is handling partially explored - grey - nodes)
-theorem dfsFindMorphismFrom_ok_correct {a: Nat} {r s: NatCDFA a} {p: Fin r.n} {q: Fin s.n}
-  {l: List (Fin a)} {asgn: DFSTable r s} (grey: List (Fin r.n))
+theorem dfsFindMorphismFrom_ok_correct {a: Nat} {r s: CDFA a} {p: r.σ} {q: s.σ}
+  {l: List (Fin a)} {asgn: DFSMap r s} (grey: List r.σ)
   (hm: okInvariant r s grey asgn):
     {fuel: Nat} → (dfsFindMorphismFrom r s p q l asgn fuel).allP (okInvariant r s grey)
   | 0 => True.intro
-  | fuel + 1 => match eq: asgn.get p with
+  | fuel + 1 => match eq: asgn[p]? with
     | none =>
-      let motive (acc: DFSResult r s) (c: Nat): Prop := acc.allP (fun acc2 =>
+      let motive (acc: Except (DFSError a) (DFSMap r s)) (c: Nat): Prop := acc.allP (fun acc2 =>
           okInvariant r s (p::grey) acc2
-          ∧ (∀ b: Fin a, b.val < c → ∃ u: List (Fin a), acc2.get (r.δ p b) = some (s.δ q b, u))
-          ∧ (∃ u: List (Fin a), acc2.get p = some (q, u))
+          ∧ (∀ b: Fin a, b.val < c → ∃ u: List (Fin a), acc2[r.δ p b]? = some (s.δ q b, u))
+          ∧ (∃ u: List (Fin a), acc2[p]? = some (q, u))
         )
       have ind: motive (Fin.foldlM a
           (fun acc b => dfsFindMorphismFrom r s (r.δ p b) (s.δ q b) (b::l) acc fuel)
-          (asgn.set p (some (q, l)))) a :=
+          (asgn.insert p (q, l))) a :=
         Fin.foldlM_induction motive
           (Except.pure_def ▸ ⟨
             fun i hi =>
                 have ne: p ≠ i := fun eq2 => hi (eq2 ▸ List.mem_cons_self)
                 have nmem: i ∉ grey := fun mem => hi (List.mem_cons_of_mem _ mem)
-                (Vector.get_set_of_ne ne).symm ▸ (Option.allP_mp (hm i nmem) (fun ⟨j, u⟩ hj b =>
+                (Std.HashMap.getElem?_insert_of_ne ne).symm ▸ (Option.allP_mp (hm i nmem) (fun ⟨j, _⟩ hj b =>
                   have ⟨uj, huj⟩ := hj b
                   have ne2: p ≠ r.δ i b := fun eq2 => (Option.some_ne_none (s.δ j b, uj))
                     (huj.symm.trans (eq2 ▸ eq))
-                  (Vector.get_set_of_ne ne2).symm ▸ hj b)),
+                  (Std.HashMap.getElem?_insert_of_ne ne2).symm ▸ hj b)),
             fun b hb => False.elim (Nat.not_lt_zero b hb),
-            ⟨l, Vector.get_set_self⟩
+            ⟨l, Std.HashMap.getElem?_insert_self⟩
           ⟩)
           (fun acc b hrec => match acc with
               | Except.error _ => True.intro
               | Except.ok acc => (
                   have prev: (dfsFindMorphismFrom r s (r.δ p b) (s.δ q b) (b::l) acc fuel).allP
-                      (fun acc2 => ∀ c: Fin a, c.val < b → ∃ u: List (Fin a), acc2.get (r.δ p c) = some (s.δ q c, u)) :=
+                      (fun acc2 => ∀ c: Fin a, c.val < b → ∃ u: List (Fin a), acc2[r.δ p c]? = some (s.δ q c, u)) :=
                     Except.allP_forall.mp (fun c => Except.allP_imp.mp (fun hc =>
                       have ⟨u, hu⟩ := hrec.right.left c hc
-                      Except.allP_mp (dfsFindMorphismFrom_preserves_some hu) (fun acc2 hacc2 => ⟨u, hacc2⟩)
+                      Except.allP_mp (dfsFindMorphismFrom_preserves hu) (fun _ hacc2 => ⟨u, hacc2⟩)
                     ))
                   Except.allP_mp (Except.allP_and.mp ⟨
                     dfsFindMorphismFrom_ok_correct (p::grey) hrec.left,
@@ -127,10 +125,10 @@ theorem dfsFindMorphismFrom_ok_correct {a: Nat} {r s: NatCDFA a} {p: Fin r.n} {q
                       Except.allP_and.mp ⟨
                         dfsFindMorphismFrom_step,
                         have ⟨u, hu⟩ := hrec.right.right;
-                        Except.allP_mp (dfsFindMorphismFrom_preserves_some hu) (fun _ hu2 => ⟨u, hu2⟩),
+                        Except.allP_mp (dfsFindMorphismFrom_preserves hu) (fun _ hu2 => ⟨u, hu2⟩),
                       ⟩
                     ⟩
-                  ⟩) (fun acc2 ⟨hrec1, hrec2, hrec3, hrec4⟩ => ⟨
+                  ⟩) (fun _ ⟨hrec1, hrec2, hrec3, hrec4⟩ => ⟨
                       hrec1,
                       (fun c hc => match Nat.lt_or_eq_of_le (Nat.le_of_lt_succ hc) with
                         | .inl lt => hrec2 c lt
@@ -144,7 +142,7 @@ theorem dfsFindMorphismFrom_ok_correct {a: Nat} {r s: NatCDFA a} {p: Fin r.n} {q
       dfsFindMorphismFrom.eq_def r s p q l asgn _ ▸ eq ▸
           Except.allP_mp ind (fun acc hacc p2 hp2 =>
             if eq2: p2 = p then
-              have ⟨u, hu⟩: ∃ u, acc.get p2 = some (q, u) := eq2 ▸ hacc.right.right
+              have ⟨_, hu⟩: ∃ u, acc[p2]? = some (q, u) := eq2 ▸ hacc.right.right
               hu ▸ fun b => eq2 ▸ hacc.right.left b b.isLt
             else
               hacc.left p2 (fun mem => match List.mem_cons.mp mem with
@@ -152,71 +150,71 @@ theorem dfsFindMorphismFrom_ok_correct {a: Nat} {r s: NatCDFA a} {p: Fin r.n} {q
                 | .inr mem2 => hp2 mem2
               )
           )
-    | some q' => dfsFindMorphismFrom.eq_def r s p q l asgn _ ▸ eq ▸
+    | some _ => dfsFindMorphismFrom.eq_def r s p q l asgn _ ▸ eq ▸
         iteInduction (motive := fun w: Except _ _ => w.allP _)
           (fun _ =>  hm) (fun _ => True.intro)
 
 
-theorem dfsFindMorphismFrom_cNone {a: Nat} {r s: NatCDFA a} {p: Fin r.n} {q: Fin s.n}
-  {l: List (Fin a)} {asgn: DFSTable r s}:
-    {fuel: Nat} → (dfsFindMorphismFrom r s p q l asgn fuel).allP (fun w => w.cNone ≤ asgn.cNone)
+theorem dfsFindMorphismFrom_size {a: Nat} {r s: CDFA a} {p: r.σ} {q: s.σ}
+  {l: List (Fin a)} {asgn: DFSMap r s}:
+    {fuel: Nat} → (dfsFindMorphismFrom r s p q l asgn fuel).allP (fun acc => acc.size ≥ asgn.size)
   | 0 => True.intro
-  | fuel + 1 =>
-    match eq: asgn.get p with
+  | _ + 1 => match eq: asgn[p]? with
     | none => dfsFindMorphismFrom.eq_def r s p q l asgn _ ▸ eq ▸
         Fin.foldlM_induction (fun (w: Except _ _) _ => w.allP _)
-          (Option.pure_def ▸ (Nat.le_of_add_le_add_right (b := 1)
-            (Vector.cNone_set eq ▸ Nat.le_succ asgn.cNone)))
-          (fun acc b hrec => match acc with
+          (Except.pure_def ▸ Std.HashMap.size_le_size_insert)
+          (fun acc _ hrec => match acc with
             | Except.error _ => True.intro
-            | Except.ok acc =>
-              have hrec2: (dfsFindMorphismFrom r s (r.δ p b) (s.δ q b) (b::l) acc fuel).allP
-                  (fun w => w.cNone ≤ acc.cNone) := dfsFindMorphismFrom_cNone
-              Except.allP_mp hrec2 (fun _ hacc2 => (Nat.le_trans hacc2 hrec))
+            | Except.ok _ =>
+              Except.allP_mp dfsFindMorphismFrom_size (fun _ h2 => Nat.le_trans hrec h2)
           )
     | some _ => dfsFindMorphismFrom.eq_def r s p q l asgn _ ▸ eq ▸
         iteInduction (motive := fun w: Except _ _ => w.allP _)
-          (fun _ => Nat.le_refl asgn.cNone) (fun _ => True.intro)
+          (fun _ => Nat.le_refl _) (fun _ => True.intro)
 
 
-def errInvariant {a: Nat} (r s: NatCDFA a) (acc: DFSTable r s): Prop :=
-    ∀ p: Fin r.n, (acc.get p).allP (fun (q, u) => r.advance u.reverse = p ∧ s.advance u.reverse = q)
+def errInvariant {a: Nat} (r s: CDFA a) (acc: DFSMap r s): Prop :=
+    ∀ p: r.σ, acc[p]?.allP (fun (q, u) => r.advance u.reverse = p ∧ s.advance u.reverse = q)
 
 
-def resultCorrect {a: Nat} {r s: NatCDFA a}: DFSResult r s → Prop
+def resultCorrect {a: Nat} {r s: CDFA a}: Except (DFSError a) (DFSMap r s) → Prop
   | Except.ok acc => errInvariant r s acc
   | Except.error (u1, u2) => r.advance u1 = r.advance u2 ∧ s.advance u1 ≠ s.advance u2
 
 
-theorem dfsFindMorphismFrom_err_correct {a: Nat} {r s: NatCDFA a} {p: Fin r.n} {q: Fin s.n}
-  {l: List (Fin a)} {asgn: DFSTable r s} (ht1: errInvariant r s asgn)
+theorem dfsFindMorphismFrom_err_correct {a: Nat} {r s: CDFA a} {p: r.σ} {q: s.σ}
+  {l: List (Fin a)} {asgn: DFSMap r s} (ht1: errInvariant r s asgn)
   (ht2: p = r.advance l.reverse ∧ q = s.advance l.reverse)
-  {fuel: Nat} (hf: fuel > asgn.cNone):
+  {fuel: Nat} (hf: fuel > FiniteHashable.cardinal r.σ - asgn.size):
     resultCorrect (dfsFindMorphismFrom r s p q l asgn fuel) :=
   match fuel with
-  | 0 => False.elim (Nat.not_lt_zero asgn.cNone hf)
+  | 0 => False.elim (Nat.not_lt_zero _ hf)
   | fuel + 1 =>
-    match eq: asgn.get p with
+    match eq: asgn[p]? with
     | none => dfsFindMorphismFrom.eq_def r s p q l asgn _ ▸ eq ▸
-        (Fin.foldlM_induction (fun res _ => resultCorrect res ∧ res.allP (fun z => fuel > z.cNone))
-          ⟨Except.pure_def ▸ fun p2 => if eq2: p2 = p then
-              congrArg (Vector.get _) eq2 ▸ Vector.get_set_self ▸ ⟨eq2 ▸ ht2.left.symm, ht2.right.symm⟩
+        (Fin.foldlM_induction (fun res _ => resultCorrect res ∧ res.allP
+            (fun z => fuel > FiniteHashable.cardinal r.σ - z.size))
+          (Except.pure_def ▸ ⟨fun p2 => if eq2: p2 = p then
+              congrArg (fun w => (asgn.insert p _)[w]?) eq2 ▸ Std.HashMap.getElem?_insert_self (α := r.σ) ▸
+                ⟨eq2 ▸ ht2.left.symm, ht2.right.symm⟩
             else
-              (Vector.get_set_of_ne (Ne.symm eq2)).symm ▸ (ht1 p2),
-            Nat.lt_of_add_lt_add_right (Vector.cNone_set eq ▸ hf),
-          ⟩
+              (Std.HashMap.getElem?_insert_of_ne (Ne.symm eq2)).symm ▸ (ht1 p2),
+            Nat.lt_of_lt_of_le (FiniteHashable.hashmap_insert_remaining_lt
+              (fun mem => nomatch (eq ▸ Std.HashMap.isSome_getElem?_iff_mem.mpr mem)))
+              (Nat.le_of_lt_succ hf)
+          ⟩)
           (fun acc _ hrec => match acc with
               | Except.error _ => hrec
               | Except.ok _ =>
                 ⟨
                   dfsFindMorphismFrom_err_correct hrec.left
                     ⟨
-                      List.reverse_cons ▸ NatCDFA.advance_concat ▸ ht2.left ▸ rfl,
-                      List.reverse_cons ▸ NatCDFA.advance_concat ▸ ht2.right ▸ rfl,
+                      List.reverse_cons ▸ CDFA.advance_concat ▸ ht2.left ▸ rfl,
+                      List.reverse_cons ▸ CDFA.advance_concat ▸ ht2.right ▸ rfl,
                     ⟩
                     hrec.right,
-                  Except.allP_mp dfsFindMorphismFrom_cNone (fun _ hacc2 =>
-                    (Nat.lt_of_le_of_lt hacc2 hrec.right))
+                  Except.allP_mp dfsFindMorphismFrom_size (fun _ hacc2 =>
+                    (Nat.lt_of_le_of_lt (Nat.sub_le_sub_left hacc2 _) hrec.right))
                 ⟩
           )
         ).left
@@ -232,144 +230,132 @@ theorem dfsFindMorphismFrom_err_correct {a: Nat} {r s: NatCDFA a} {p: Fin r.n} {
           )
 
 /-
-Non-recursive (simpler) version
+Non-recursive version
 -/
-def dfsFindMorphism {a: Nat} (r s: NatCDFA a): DFSResult r s :=
-  dfsFindMorphismFrom r s r.i s.i [] (Vector.replicate r.n none) (r.n + 1)
+def dfsFindMorphism {a: Nat} (r s: CDFA a): Except (DFSError a) (DFSMap r s) :=
+  dfsFindMorphismFrom r s r.i s.i [] ∅ (FiniteHashable.cardinal r.σ + 1)
 
 
-def allP_of_resultCorrect {a: Nat} {r s: NatCDFA a} {res: DFSResult r s} (h: resultCorrect res):
+def allP_of_resultCorrect {a: Nat} {r s: CDFA a} {res: Except (DFSError a) (DFSMap r s)}
+  (h: resultCorrect res):
     res.allP (errInvariant r s) :=
   match res with
   | Except.ok _ => h
   | Except.error _ => True.intro
 
 
-theorem dfsFindMorphism_ok_correct {a: Nat} {r s: NatCDFA a}:
+theorem dfsFindMorphism_ok_correct {a: Nat} {r s: CDFA a}:
     (dfsFindMorphism r s).allP (fun acc =>
-      (∀ p: Fin r.n, (acc.get p).allP (fun (_, l) => r.advance l.reverse = p))
-      ∧ (∀ l: List (Fin a), ∃ u: List (Fin a), acc.get (r.advance l) = some (s.advance l, u))
+      (∀ p: r.σ, acc[p]?.allP (fun (_, l) => r.advance l.reverse = p))
+      ∧ (∀ l: List (Fin a), ∃ u: List (Fin a), acc[r.advance l]? = some (s.advance l, u))
     ) :=
   Except.allP_mp (Except.allP_and.mp ⟨
-    dfsFindMorphismFrom_ok_correct [] (fun p _ => Vector.get_replicate ▸ True.intro),
+    dfsFindMorphismFrom_ok_correct [] (fun p _ => Std.HashMap.getElem?_empty ▸ True.intro),
     Except.allP_and.mp ⟨
       allP_of_resultCorrect (dfsFindMorphismFrom_err_correct
-        (fun p => Vector.get_replicate ▸ True.intro)
+        (fun p => Std.HashMap.getElem?_empty ▸ True.intro)
         ⟨Array.toList_empty ▸ rfl, Array.toList_empty ▸ rfl⟩
-        (Nat.lt_succ_of_le Vector.cNone_le)
+        (Std.HashMap.size_empty ▸ Nat.sub_zero _ ▸ Nat.lt_add_one (FiniteHashable.cardinal r.σ))
       ),
       dfsFindMorphismFrom_step
     ⟩
   ⟩) (fun acc ⟨hacc1, hacc2, hacc3⟩ => ⟨
     (fun p => Option.allP_mp (hacc2 p) (fun (q, u) h => h.left)),
-    let rec propagate (l: List (Fin a)): ∃ u, acc.get (r.advance l) = some (s.advance l, u) :=
+    let rec propagate (l: List (Fin a)): ∃ u, acc[r.advance l]? = some (s.advance l, u) :=
       match List.eq_nil_or_concat l with
       | .inl eq_nil => eq_nil ▸ hacc3
       | .inr ⟨start, b, eq_cat⟩ =>
         have ⟨u, hrec⟩ := propagate start
-        have inv: (acc.get (r.advance start)).allP
-            (fun (q, _) => ∀ c: Fin a, ∃ u, acc.get (r.δ (r.advance start) c) = some (s.δ q c, u)) :=
+        have inv: acc[r.advance start]?.allP
+            (fun (q, _) => ∀ c: Fin a, ∃ u, acc[r.δ (r.advance start) c]? = some (s.δ q c, u)) :=
           hacc1 (r.advance start) List.not_mem_nil
-        have invs: ∀ (c : Fin a), ∃ u, acc.get (r.δ (r.advance start) c) = some (s.δ (s.advance start) c, u) :=
+        have invs: ∀ (c : Fin a), ∃ u, acc[r.δ (r.advance start) c]? = some (s.δ (s.advance start) c, u) :=
           hrec.subst inv
         have hr: r.advance l = r.δ (r.advance start) b :=
-          eq_cat ▸ List.concat_eq_append ▸ NatCDFA.advance_concat
+          eq_cat ▸ List.concat_eq_append ▸ CDFA.advance_concat
         have hs: s.advance l = s.δ (s.advance start) b :=
-          eq_cat ▸ List.concat_eq_append ▸ NatCDFA.advance_concat
+          eq_cat ▸ List.concat_eq_append ▸ CDFA.advance_concat
         hr ▸ hs ▸ invs b
       termination_by l.length
     propagate
   ⟩)
 
 
-theorem dfsFindMorphism_err_correct {a: Nat} {r s: NatCDFA a}:
+theorem dfsFindMorphism_err_correct {a: Nat} {r s: CDFA a}:
     (dfsFindMorphism r s).allEP (fun (l1, l2) =>
       r.advance l1 = r.advance l2 ∧ s.advance l1 ≠ s.advance l2) :=
   match eq: dfsFindMorphism r s with
   | Except.error (_, _) =>
     have res_correct: resultCorrect (dfsFindMorphism r s) :=
       dfsFindMorphismFrom_err_correct
-        (fun _ => Vector.get_replicate ▸ True.intro)
+        (fun _ => Std.HashMap.getElem?_empty ▸ True.intro)
         ⟨Array.toList_empty ▸ rfl, Array.toList_empty ▸ rfl⟩
-        (Nat.lt_succ_of_le Vector.cNone_le)
+        (Std.HashMap.size_empty ▸ Nat.sub_zero _ ▸ Nat.lt_add_one (FiniteHashable.cardinal r.σ))
     have concl := eq.subst res_correct; concl
   | Except.ok _ => True.intro
-
 
 /-
 Construction over the previous function to search for a true morphism (or provide a counterexample)
 -/
-def checkTerminal {a: Nat} (r s: NatCDFA a) (m: DFSTable r s): Except (List (Fin a)) Unit :=
-  Fin.foldlM r.n (fun () p =>
-    match m.get p with
-    | none => Except.ok ()
-    | some (q, u) => if s.f q = r.f p then Except.ok () else Except.error u.reverse
-  ) ()
+def checkTerminal {a: Nat} (r s: CDFA a) (m: DFSMap r s): Except (List (Fin a)) Unit :=
+  m.forM (fun p (q, u) => if s.f q = r.f p then Except.ok () else Except.error u.reverse)
 
 
-def checkTerminal_ok_correct {a: Nat} {r s: NatCDFA a} {m: DFSTable r s}:
-    (checkTerminal r s m).allP (fun () => ∀ p: Fin r.n, (m.get p).allP (fun (q, _) => r.f p = s.f q)) :=
-  let motive (acc: Except (List (Fin a)) Unit) (i: Nat) :=
-    acc.allP (fun () => ∀ p: Fin r.n, p < i → (m.get p).allP (fun (q, _) => r.f p = s.f q))
-  have ind: motive (checkTerminal r s m) r.n := Fin.foldlM_induction motive
-    (Except.pure_def ▸ fun p hp => False.elim (Nat.not_lt_zero p hp))
-    (fun acc i hrec => match acc with
-      | Except.error _ => True.intro
-      | Except.ok _ => match eq: m.get i with
-        | none =>
-          have concl: ∀ p: Fin r.n, p < i.val.succ → (m.get p).allP (fun (q, _) => r.f p = s.f q) :=
-            fun p hp => match Nat.lt_or_eq_of_le (Nat.le_of_lt_succ hp) with
-              | Or.inl lt => hrec p lt
-              | Or.inr eq2 => Fin.eq_of_val_eq eq2 ▸ eq ▸ True.intro
-          concl
-        | some (_, _) => iteInduction (motive := fun acc => motive acc i.val.succ)
-          (fun eq2 =>
-            have concl: ∀ p: Fin r.n, p < i.val.succ → (m.get p).allP (fun (q, _) => r.f p = s.f q) :=
-            fun p hp => match Nat.lt_or_eq_of_le (Nat.le_of_lt_succ hp) with
-              | Or.inl lt => hrec p lt
-              | Or.inr eq3 => Fin.eq_of_val_eq eq3 ▸ eq ▸ eq2.symm
-            concl )
-          (fun _ => True.intro)
-    )
-  Except.allP_mp ind (fun () h p => h p p.isLt)
+theorem checkTerminal_ok_correct {a: Nat} {r s: CDFA a} {m: DFSMap r s}:
+    (checkTerminal r s m).allP (fun () => ∀ p: r.σ, m[p]?.allP (fun (q, _) => r.f p = s.f q)) :=
+  checkTerminal.eq_def r s m ▸
+  Std.HashMap.forM_eq_forM (m' := Except _) ▸
+  Std.HashMap.forM_eq_forM_toList (m' := Except _) ▸
+  List.forM_eq_forM (m := Except _) ▸
+  Except.allP_mp List.forM_ok (fun () h p => match eq: m[p]? with
+    | none => True.intro
+    | some (q, l) =>
+      have concl: r.f p = s.f q := if eq2: r.f p = s.f q then eq2 else
+        nomatch (ite_eq_left_iff.mp (h (p, (q, l))
+          (Std.HashMap.mem_toList_iff_getElem?_eq_some.mpr eq)) (Ne.symm eq2))
+      concl
+  )
 
 
-def checkTerminal_err_correct {a: Nat} {r s: NatCDFA a} {m: DFSTable r s}:
+theorem checkTerminal_err_correct {a: Nat} {r s: CDFA a} {m: DFSMap r s}:
     (checkTerminal r s m).allEP (fun l =>
-      ∃ p: Fin r.n, ∃ q: Fin s.n, (m.get p) = some (q, l.reverse) ∧ s.f q ≠ r.f p) :=
-  Fin.foldlM_induction (motive := fun (acc: Except _ _) _ => acc.allEP _)
-    (Except.pure_def ▸ True.intro)
-    (fun acc p hrec => match acc with
-      | Except.error _ => hrec
-      | Except.ok _ => match eq: Vector.get m p with
-        | none => True.intro
-        | some (q, _) => iteInduction (fun _ => True.intro)
-          (fun ne => ⟨p, q, List.reverse_reverse _ ▸ eq, ne⟩)
-    )
+      ∃ (p: r.σ) (q: s.σ), m[p]? = some (q, l.reverse) ∧ s.f q ≠ r.f p) :=
+  checkTerminal.eq_def r s m ▸
+  Std.HashMap.forM_eq_forM (m' := Except _) ▸
+  Std.HashMap.forM_eq_forM_toList (m' := Except _) ▸
+  List.forM_eq_forM (m := Except _) ▸
+  Except.allEP_mp List.forM_error (fun l ⟨(p, q, u), mem, eq⟩ =>
+    if eq2: r.f p = s.f q then
+      nomatch (eq.symm.trans (if_pos eq2.symm))
+    else
+      have h: l = u.reverse := Except.error.inj (eq.symm.trans (if_neg (Ne.symm eq2)))
+      have h2: l.reverse = u := List.reverse_reverse u ▸ congrArg List.reverse h
+      ⟨p, q, Std.HashMap.mem_toList_iff_getElem?_eq_some.mp (h2 ▸ mem), Ne.symm eq2⟩
+  )
 
 
 /-
 The final, clean API
 -/
 public section
-namespace NatCDFA
+namespace CDFA
 
-inductive MorphismObstruction {a: Nat} (r s: NatCDFA a) where
+inductive MorphismObstruction {a: Nat} (r s: CDFA a) where
   | state: (l1: List (Fin a)) → (l2: List (Fin a)) →
     (r.advance l1 = r.advance l2) → (s.advance l1 ≠ s.advance l2) → MorphismObstruction r s
   | final: (l: List (Fin a)) → r.accepts l ≠ s.accepts l → MorphismObstruction r s
 
 
-inductive FindMorphismResult {a: Nat} (r s: NatCDFA a) where
-  | morphism: (f: Fin r.n → Fin s.n) → (NatCDFA.morphism r s f) → FindMorphismResult r s
+inductive FindMorphismResult {a: Nat} (r s: CDFA a) where
+  | morphism: (f: r.σ → s.σ) → (CDFA.morphism r s f) → FindMorphismResult r s
   | obstruction: MorphismObstruction r s → FindMorphismResult r s
 
 
-def findMorphism {a: Nat} (r s: NatCDFA a): FindMorphismResult r s :=
+def findMorphism {a: Nat} (r s: CDFA a): FindMorphismResult r s :=
   match eq: dfsFindMorphism r s with
   | Except.ok acc => have h := eq ▸ dfsFindMorphism_ok_correct (r := r) (s := s)
     match eq2: checkTerminal r s acc with
-    | Except.ok () => FindMorphismResult.morphism (fun i => (((acc.get i).map Prod.fst).getD s.i))
+    | Except.ok () => FindMorphismResult.morphism (fun i => ((acc[i]?.map Prod.fst).getD s.i))
       (fun l => have ⟨_, eqm⟩ := h.right l
         ⟨
           (congrArg (fun opt => (opt.map Prod.fst).getD s.i) eqm).trans rfl,
@@ -390,7 +376,48 @@ def findMorphism {a: Nat} (r s: NatCDFA a): FindMorphismResult r s :=
     FindMorphismResult.obstruction (MorphismObstruction.state l1 l2 h.left h.right)
 
 
-theorem not_existsMorphism_of_obstruction {a: Nat} {r s: NatCDFA a} (obstruction: MorphismObstruction r s):
+theorem not_existsMorphism_of_obstruction {a: Nat} {r s: CDFA a}
+  (obstruction: MorphismObstruction r s):
+    ¬CDFA.existsMorphism r s :=
+  fun ⟨f, hf⟩ => match obstruction with
+  | MorphismObstruction.state l1 l2 hr hs =>
+    hs (((hf l1).left.symm.trans (congrArg f hr)).trans (hf l2).left)
+  | MorphismObstruction.final l hl => hl (hf l).right
+
+end CDFA
+
+/-
+NatCDFA version
+-/
+namespace NatCDFA
+
+inductive MorphismObstruction {a: Nat} (r s: NatCDFA a) where
+  | state: (l1: List (Fin a)) → (l2: List (Fin a)) →
+    (r.advance l1 = r.advance l2) → (s.advance l1 ≠ s.advance l2) → MorphismObstruction r s
+  | final: (l: List (Fin a)) → r.accepts l ≠ s.accepts l → MorphismObstruction r s
+
+
+inductive FindMorphismResult {a: Nat} (r s: NatCDFA a) where
+  | morphism: (f: Fin r.n → Fin s.n) → (NatCDFA.morphism r s f) → FindMorphismResult r s
+  | obstruction: MorphismObstruction r s → FindMorphismResult r s
+
+
+def findMorphism {a: Nat} (r s: NatCDFA a): FindMorphismResult r s :=
+  let result: CDFA.FindMorphismResult r.toCDFA s.toCDFA := CDFA.findMorphism r.toCDFA s.toCDFA
+  match result with
+  | CDFA.FindMorphismResult.morphism f h => FindMorphismResult.morphism f
+    (NatCDFA.morphism_toCDFA.mpr h)
+  | CDFA.FindMorphismResult.obstruction obstruction => FindMorphismResult.obstruction (
+    match obstruction with
+    | CDFA.MorphismObstruction.state l1 l2 eq ne => MorphismObstruction.state l1 l2
+      (advance_toCDFA ▸ advance_toCDFA ▸ eq) (advance_toCDFA ▸ advance_toCDFA ▸ ne)
+    | CDFA.MorphismObstruction.final l ne => MorphismObstruction.final l
+      (accepts_toCDFA ▸ accepts_toCDFA ▸ ne)
+  )
+
+
+theorem not_existsMorphism_of_obstruction {a: Nat} {r s: NatCDFA a}
+  (obstruction: MorphismObstruction r s):
     ¬NatCDFA.existsMorphism r s :=
   fun ⟨f, hf⟩ => match obstruction with
   | MorphismObstruction.state l1 l2 hr hs =>
