AutoKchp/Search.lean
@@ -8,179 +8,168 @@ module
 
 public import AutoKchp.CDFA
 import AutoKchp.Internal.Util
+import Std.Data.HashSet
 
 
-def dfsFrom {a: Nat} (r: NatCDFA a) (p: Fin r.n)
-  (l: List (Fin a)) (visited: Vector Bool r.n):
-    Nat → Except (List (Fin a)) (Vector Bool r.n)
+def dfsFrom {a: Nat} (r: CDFA a) (p: r.σ) (l: List (Fin a)) (visited: Std.HashSet r.σ):
+    Nat → Except (List (Fin a)) (Std.HashSet r.σ)
   | 0 => Except.error []
   | fuel + 1 =>
-    if visited.get p then Except.ok visited
+    if visited.contains p then Except.ok visited
     else if r.f p then Except.error l.reverse
     else Fin.foldlM a
       (fun acc b => dfsFrom r (r.δ p b) (b::l) acc fuel)
-      (visited.set p true)
+      (visited.insert p)
 
 
-theorem dfsFrom_preserves_true {a: Nat} {r: NatCDFA a} {p: Fin r.n} {l: List (Fin a)}
-  {visited: Vector Bool r.n} {i: Fin r.n} (h: visited.get i = true):
-    {fuel: Nat} → (dfsFrom r p l visited fuel).allP (fun acc => acc.get i = true)
+theorem dfsFrom_preserves_mem {a: Nat} {r: CDFA a} {p: r.σ} {l: List (Fin a)}
+  {visited: Std.HashSet r.σ} {i: r.σ} (h: i ∈ visited):
+    {fuel: Nat} → (dfsFrom r p l visited fuel).allP (fun acc => i ∈ acc)
   | 0 => True.intro
-  | _ + 1 => iteInduction (fun _ => h) (fun nv => iteInduction
+  | _ + 1 => iteInduction (fun _ => h) (fun _ => iteInduction
     (fun _ => True.intro) (fun _ => Fin.foldlM_induction
       (fun (w: Except _ _) _ => w.allP _)
-      (have ne2: p ≠ i := fun eq => nv (eq ▸ h);
-        Except.pure_def ▸ (Vector.get_set_of_ne ne2).trans h)
+      (Except.pure_def ▸ Std.HashSet.mem_insert.mpr (Or.inr h))
       (fun acc _ hrec => match acc with
         | Except.error _ => True.intro
-        | Except.ok _ => dfsFrom_preserves_true hrec
+        | Except.ok _ => dfsFrom_preserves_mem hrec
       )
     ))
 
 
-theorem dfsFrom_step {a: Nat} {r: NatCDFA a} {p: Fin r.n} {l: List (Fin a)}
-  {visited: Vector Bool r.n}:
-    {fuel: Nat} → (dfsFrom r p l visited fuel).allP (fun acc => acc.get p = true)
+theorem dfsFrom_step {a: Nat} {r: CDFA a} {p: r.σ} {l: List (Fin a)}
+  {visited: Std.HashSet r.σ}:
+    {fuel: Nat} → (dfsFrom r p l visited fuel).allP (fun acc => p ∈ acc)
   | 0 => True.intro
   | _ + 1 => iteInduction (fun v => v) (fun _ => iteInduction
     (fun _ => True.intro) (fun _ => Fin.foldlM_induction
       (fun (w: Except _ _) _ => w.allP _)
-      (Except.pure_def ▸ Vector.get_set_self)
+      (Except.pure_def ▸ Std.HashSet.mem_insert_self)
       (fun acc _ hrec => match acc with
         | Except.error _ => True.intro
-        | Except.ok _ => dfsFrom_preserves_true hrec)
+        | Except.ok _ => dfsFrom_preserves_mem hrec)
     ))
 
 
-def okInvariant {a: Nat} (r: NatCDFA a)
-  (grey: List (Fin r.n)) (acc: Vector Bool r.n): Prop :=
-    ∀ p: Fin r.n, p ∉ grey → acc.get p = true → (¬r.f p ∧ (∀ b: Fin a, acc.get (r.δ p b) = true))
+def okInvariant {a: Nat} (r: CDFA a)
+  (grey: List r.σ) (acc: Std.HashSet r.σ): Prop :=
+    ∀ p: r.σ, p ∉ grey → p ∈ acc → (¬r.f p ∧ (∀ b: Fin a, r.δ p b ∈ acc))
 
 
-theorem dfsFrom_ok_correct {a: Nat} {r: NatCDFA a} {p: Fin r.n} {l: List (Fin a)}
-  {visited: Vector Bool r.n} (grey: List (Fin r.n)) (h: okInvariant r grey visited):
+theorem dfsFrom_ok_correct {a: Nat} {r: CDFA a} {p: r.σ} {l: List (Fin a)}
+  {visited: Std.HashSet r.σ} (grey: List r.σ) (h: okInvariant r grey visited):
     {fuel: Nat} → (dfsFrom r p l visited fuel).allP (okInvariant r grey)
   | 0 => True.intro
   | fuel + 1 => iteInduction (fun _ => h)
-    (fun nv => iteInduction (fun _ => True.intro)
+    (fun _ => iteInduction (fun _ => True.intro)
       (fun nf =>
         let motive acc c := acc.allP (fun acc2 =>
           okInvariant r (p::grey) acc2
-          ∧ ∀ b: Fin a, b < c → acc2.get (r.δ p b) = true
+          ∧ ∀ b: Fin a, b < c →  r.δ p b ∈ acc2
         )
         have ind: motive (Fin.foldlM a
-            (fun acc b => dfsFrom r (r.δ p b) (b::l) acc fuel) (visited.set p true)) a :=
+            (fun acc b => dfsFrom r (r.δ p b) (b::l) acc fuel) (visited.insert p)) a :=
           Fin.foldlM_induction motive
             (Except.pure_def ▸ ⟨
               fun p2 hp2 vp2 =>
                 have ne: p ≠ p2 := (fun eq => hp2 (eq ▸ List.mem_cons_self))
                 have nmem: p2 ∉ grey := (fun mem => hp2 (List.mem_cons_of_mem _ mem))
-                have ⟨hl, hr⟩ := h p2 nmem ((Vector.get_set_of_ne ne) ▸ vp2)
+                have ⟨hl, hr⟩ := h p2 nmem (Std.HashSet.mem_of_mem_insert vp2 (beq_eq_false_iff_ne.mpr ne))
                 ⟨
                   hl,
-                  fun b =>
-                    have ne2: p ≠ r.δ p2 b := fun eq2 => (nv (eq2 ▸ hr b))
-                    (Vector.get_set_of_ne ne2).symm ▸ (hr b)
+                  fun b => Std.HashSet.mem_insert.mpr (Or.inr (hr b))
                 ⟩,
               fun b hb => False.elim (Nat.not_lt_zero b hb)
             ⟩)
-            (fun acc b hrec => match acc with
+            (fun acc _ hrec => match acc with
               | Except.error _ => True.intro
-              | Except.ok acc => Except.allP_and.mp ⟨
+              | Except.ok _ => Except.allP_and.mp ⟨
                 dfsFrom_ok_correct (p::grey) hrec.left,
                 Except.allP_forall.mp (fun c => Except.allP_imp.mp (fun hc =>
                   match Nat.lt_or_eq_of_le (Nat.le_of_lt_succ hc) with
-                  | .inl lt => dfsFrom_preserves_true (hrec.right c lt)
+                  | .inl lt => dfsFrom_preserves_mem (hrec.right c lt)
                   | .inr eq => Fin.eq_of_val_eq eq ▸ dfsFrom_step
                 ))
               ⟩
             )
-        Except.allP_mp ind (fun acc ⟨hacc1, hacc2⟩ p2 hp2 v =>
-          if eq: p2 = p then ⟨eq ▸ nf, fun b => eq ▸ hacc2 b b.isLt⟩
-          else hacc1 p2 (fun mem => hp2 ((List.mem_cons.mp mem).resolve_left eq)) v
+        Except.allP_mp ind (fun _ ⟨hacc1, hacc2⟩ p2 hp2 v =>
+          if eq: p2 == p then ⟨eq_of_beq eq ▸ nf, fun b => eq_of_beq eq ▸ hacc2 b b.isLt⟩
+          else hacc1 p2 (fun mem => hp2 ((List.mem_cons.mp mem).resolve_left (ne_of_beq_false (eq_false_of_ne_true eq)))) v
         )
       ))
 
 
-theorem count_true_set {k: Nat} {v: Vector Bool k} {i: Fin k}
-  (h: v.get i = false):
-    (v.set i true).count false + 1 = v.count false :=
-  have cond1: ((v[i.val] == false) = true) = True := eq_true (Bool.beq_to_eq v[i.val] _ ▸ h)
-  have cond2: ((true == false) = true) = False := eq_false (fun eq => nomatch eq)
-  have le: v.count false ≥ 1 := Nat.one_le_of_lt (Vector.count_pos_iff.mpr (h ▸ Vector.get_mem))
-  (congrArg (· + 1) (Vector.count_set i.isLt)).trans (
-    (ite_cond_eq_true 1 0 cond1).symm ▸ (ite_cond_eq_false 1 0 cond2).symm ▸
-      Nat.sub_add_cancel le)
-
-
-theorem dfsFrom_count {a: Nat} {r: NatCDFA a} {p: Fin r.n}
-  {l: List (Fin a)} {visited: Vector Bool r.n}:
-    {fuel: Nat} → (dfsFrom r p l visited fuel).allP (fun acc => acc.count false ≤ visited.count false)
+theorem dfsFrom_size {a: Nat} {r: CDFA a} {p: r.σ}
+  {l: List (Fin a)} {visited: Std.HashSet r.σ}:
+    {fuel: Nat} → (dfsFrom r p l visited fuel).allP (fun acc => acc.size ≥ visited.size)
   | 0 => True.intro
-  | _ + 1 => iteInduction (fun _ => Nat.le_refl _) (fun h => iteInduction
+  | _ + 1 => iteInduction (fun _ => Nat.le_refl _) (fun _ => iteInduction
     (fun _ => True.intro)
     (fun _ => Fin.foldlM_induction
-      (fun (acc: Except _ (Vector Bool r.n)) _ => acc.allP
-        (fun acc2 => acc2.count false ≤ visited.count false))
-      (Except.pure_def ▸ Nat.le_of_add_le_add_right
-        (Nat.le_trans (Nat.le_of_eq (count_true_set (Bool.not_eq_true _ ▸ h))) (Nat.le_succ _)))
+      (fun (acc: Except _ (Std.HashSet r.σ)) _ => acc.allP
+        (fun acc2 => acc2.size ≥ visited.size))
+      (Except.pure_def ▸ Std.HashSet.size_le_size_insert)
       (fun acc _ hrec => match acc with
         | Except.error _ => True.intro
-        | Except.ok _ => Except.allP_mp dfsFrom_count (fun _ h2 => Nat.le_trans h2 hrec)
+        | Except.ok _ => Except.allP_mp dfsFrom_size (fun _ h2 => Nat.le_trans hrec h2)
       )
     ))
 
 
-theorem dfsFrom_err_correct {a: Nat} {r: NatCDFA a} {p: Fin r.n} {l: List (Fin a)}
-  {visited: Vector Bool r.n} (h: p = r.advance l.reverse):
-    {fuel: Nat} → fuel > visited.count false → (dfsFrom r p l visited fuel).allEP (fun u => r.accepts u)
+theorem dfsFrom_err_correct {a: Nat} {r: CDFA a} {p: r.σ} {l: List (Fin a)}
+  {visited: Std.HashSet r.σ} (h: p = r.advance l.reverse):
+    {fuel: Nat} → fuel > FiniteHashable.cardinal r.σ - visited.size →
+      (dfsFrom r p l visited fuel).allEP (fun u => r.accepts u)
   | 0 => fun hf => False.elim (Nat.not_lt_zero _ hf)
   | fuel + 1 => fun hf =>
     iteInduction (fun _ => True.intro) (fun nv => iteInduction
       (fun h2 => have concl: r.f (r.advance l.reverse) = true := h ▸ h2; concl)
       (fun _ => (Fin.foldlM_induction
-        (fun (w: Except _ _) _ => w.allEP (fun u => r.accepts u) ∧ w.allP (fun acc => fuel > acc.count false))
+        (fun (w: Except _ _) _ => w.allEP (fun u => r.accepts u) ∧ w.allP
+          (fun acc => fuel > FiniteHashable.cardinal r.σ - acc.size))
         (Except.pure_def ▸ ⟨True.intro,
-          Nat.lt_of_add_lt_add_right ((count_true_set (Bool.not_eq_true _ ▸ nv)) ▸ hf)⟩)
+            Nat.lt_of_lt_of_le (FiniteHashable.hashset_insert_remaining_lt nv) (Nat.le_of_lt_succ hf)
+          ⟩)
         (fun acc _ hrec => match acc with
           | Except.error _ => hrec
           | Except.ok _ => ⟨
               dfsFrom_err_correct
-                (h ▸ List.reverse_cons ▸ NatCDFA.advance_concat.symm)
+                (h ▸ List.reverse_cons ▸ CDFA.advance_concat.symm)
                 hrec.right,
-              Except.allP_mp dfsFrom_count (fun _ le => Nat.lt_of_le_of_lt le hrec.right)
+              Except.allP_mp dfsFrom_size (fun _ le => Nat.lt_of_le_of_lt
+                (Nat.sub_le_sub_left le _) hrec.right)
             ⟩
         )).left
       )
     )
 
 
-def dfs {a: Nat} (r: NatCDFA a): Option (List (Fin a)) :=
-  match dfsFrom r r.i [] (Vector.replicate r.n false) (r.n + 1) with
+def dfs {a: Nat} (r: CDFA a): Option (List (Fin a)) :=
+  match dfsFrom r r.i [] ∅ (FiniteHashable.cardinal r.σ + 1) with
   | Except.error l => some l
   | Except.ok _ => none
 
 
-theorem dfs_some_correct {a: Nat} {r: NatCDFA a}: (dfs r).all r.accepts :=
-  have concl: (dfsFrom r r.i [] (Vector.replicate r.n false) (r.n + 1)).allEP (fun u => r.accepts u) :=
-    dfsFrom_err_correct (rfl: r.i = r.advance [].reverse) (Nat.lt_succ_of_le (Vector.count_le_size))
-  match eq: dfsFrom r r.i [] (Vector.replicate r.n false) (r.n + 1) with
+theorem dfs_some_correct {a: Nat} {r: CDFA a}: (dfs r).all r.accepts :=
+  have concl: (dfsFrom r r.i [] ∅ (FiniteHashable.cardinal r.σ + 1)).allEP (fun u => r.accepts u) :=
+    dfsFrom_err_correct (rfl: r.i = r.advance [].reverse) (Std.HashSet.size_empty ▸ Nat.le_refl _)
+  match eq: dfsFrom r r.i [] ∅ (FiniteHashable.cardinal r.σ + 1) with
   | Except.ok _ => dfs.eq_def r ▸ eq ▸ rfl
   | Except.error _ => dfs.eq_def r ▸ eq ▸ concl
 
 
-theorem dfs_none_correct {a: Nat} {r: NatCDFA a} (h: dfs r = none):
+theorem dfs_none_correct {a: Nat} {r: CDFA a} (h: dfs r = none):
     ∀ l: List (Fin a), r.accepts l = false :=
-  match eq: dfsFrom r r.i [] (Vector.replicate r.n false) (r.n + 1) with
-    | Except.ok table =>
-      have h: okInvariant r [] table := eq.subst (dfsFrom_ok_correct [] (fun _ _ v =>
-          False.elim (Bool.false_ne_true (Vector.get_replicate.symm.trans v))))
-      have hs: table.get r.i = true := eq.subst dfsFrom_step
-      let rec propagate (u: List (Fin a)): table.get (r.advance u) = true :=
+  match eq: dfsFrom r r.i [] ∅ (FiniteHashable.cardinal r.σ + 1) with
+    | Except.ok visited =>
+      have h: okInvariant r [] visited := eq.subst (dfsFrom_ok_correct [] (fun _ _ v =>
+          False.elim (Std.HashSet.not_mem_empty v)))
+      have hs: r.i ∈ visited := eq.subst dfsFrom_step
+      let rec propagate (u: List (Fin a)): (r.advance u) ∈ visited :=
         match List.eq_nil_or_concat u with
         | .inl eq2 => eq2 ▸ hs
         | .inr ⟨s, b, eq2⟩ =>
-          eq2 ▸ List.concat_eq_append ▸ NatCDFA.advance_concat ▸
+          eq2 ▸ List.concat_eq_append ▸ CDFA.advance_concat ▸
             (h (r.advance s) List.not_mem_nil (propagate s)).right b
         termination_by u.length
       fun l => Bool.not_eq_true _ ▸ (h (r.advance l) List.not_mem_nil (propagate l)).left
@@ -188,14 +177,14 @@ theorem dfs_none_correct {a: Nat} {r: NatCDFA a} (h: dfs r = none):
 
 
 public section
-namespace NatCDFA
+namespace CDFA
 
-inductive SearchResult {a: Nat} (r: NatCDFA a) where
+inductive SearchResult {a: Nat} (r: CDFA a) where
   | word: (l: List (Fin a)) → r.accepts l = true → SearchResult r
   | empty: (∀ l: List (Fin a), r.accepts l = false) → SearchResult r
 
 
-def search {a: Nat} (r: NatCDFA a): SearchResult r :=
+def search {a: Nat} (r: CDFA a): SearchResult r :=
   match eq: dfs r with
   | some w => SearchResult.word w (
       have concl: Option.all r.accepts (some w) := eq ▸ dfs_some_correct
@@ -203,5 +192,5 @@ def search {a: Nat} (r: NatCDFA a): SearchResult r :=
     )
   | none => SearchResult.empty (dfs_none_correct eq)
 
-end NatCDFA
+end CDFA
 end
